src/Dafny/examples/fs/byte_fs.dfy
@@ -283,8 +283,8 @@ module ByteFs {
       calc {
         inode_data(d');
         (C.concat(C.without_last(blks')) + C.last(blks'))[..d'.sz];
-        C.concat(C.without_last(blks')) + block_to_seq(C.last(blks'))[..d'.sz - (|blks'|-1) * 4096];
-        C.concat(C.without_last(blks)) + block_to_seq(C.last(blks'))[..d'.sz - (|blks'|-1) * 4096];
+        C.concat(C.without_last(blks')) + to_seq(C.last(blks'))[..d'.sz - (|blks'|-1) * 4096];
+        C.concat(C.without_last(blks)) + to_seq(C.last(blks'))[..d'.sz - (|blks'|-1) * 4096];
       }
     }
 
